Switch to a more precise version of interp_related for rewrites
This version is hopefully the right one.  It seems to be basically
exactly what we want to say, and no more and no less.  The rule for
let-ins, which is almost the only freedom we have here, is chosen to
match exactly with the rule for App+Abs.  Note that using Leibniz
equality is essential in the places where it's used.  The recursive
relation here might actually be a bit clearer as an inductive relation,
but I wanted it to simplify under reduction.

After     | File Name                                                            | Before    || Change    | % Change
--------------------------------------------------------------------------------------------------------------------
30m04.79s | Total                                                                | 29m51.25s || +0m13.54s | +0.75%
--------------------------------------------------------------------------------------------------------------------
1m53.11s  | Experiments/NewPipeline/RewriterRulesInterpGood.vo                   | 1m35.74s  || +0m17.36s | +18.14%
0m19.40s  | Experiments/NewPipeline/RewriterWf1.vo                               | 0m24.54s  || -0m05.14s | -20.94%
6m13.78s  | Experiments/NewPipeline/SlowPrimeSynthesisExamples.vo                | 6m14.86s  || -0m01.08s | -0.28%
4m39.23s  | Experiments/NewPipeline/Toplevel1.vo                                 | 4m38.21s  || +0m01.02s | +0.36%
1m31.62s  | Experiments/NewPipeline/Toplevel2.vo                                 | 1m32.68s  || -0m01.06s | -1.14%
0m40.01s  | Experiments/NewPipeline/AbstractInterpretationWf.vo                  | 0m38.77s  || +0m01.23s | +3.19%
3m19.74s  | p384_32.c                                                            | 3m19.71s  || +0m00.03s | +0.01%
1m58.86s  | Experiments/NewPipeline/RewriterWf2.vo                               | 1m58.30s  || +0m00.56s | +0.47%
1m02.04s  | Experiments/NewPipeline/RewriterRulesGood.vo                         | 1m02.41s  || -0m00.36s | -0.59%
0m40.71s  | p521_32.c                                                            | 0m40.51s  || +0m00.20s | +0.49%
0m39.90s  | Experiments/NewPipeline/ExtractionHaskell/word_by_word_montgomery    | 0m39.85s  || +0m00.04s | +0.12%
0m36.76s  | Experiments/NewPipeline/Rewriter.vo                                  | 0m36.81s  || -0m00.05s | -0.13%
0m35.34s  | Experiments/NewPipeline/LanguageInversion.vo                         | 0m35.16s  || +0m00.18s | +0.51%
0m33.80s  | p521_64.c                                                            | 0m33.82s  || -0m00.02s | -0.05%
0m28.97s  | Experiments/NewPipeline/GENERATEDIdentifiersWithoutTypesProofs.vo    | 0m29.54s  || -0m00.57s | -1.92%
0m27.65s  | Experiments/NewPipeline/LanguageWf.vo                                | 0m28.11s  || -0m00.46s | -1.63%
0m25.94s  | Experiments/NewPipeline/ExtractionHaskell/unsaturated_solinas        | 0m25.39s  || +0m00.55s | +2.16%
0m25.63s  | Experiments/NewPipeline/UnderLetsProofs.vo                           | 0m25.15s  || +0m00.48s | +1.90%
0m22.84s  | Experiments/NewPipeline/AbstractInterpretationZRangeProofs.vo        | 0m23.11s  || -0m00.26s | -1.16%
0m18.51s  | Experiments/NewPipeline/ExtractionHaskell/saturated_solinas          | 0m18.69s  || -0m00.17s | -0.96%
0m17.42s  | Experiments/NewPipeline/AbstractInterpretationProofs.vo              | 0m17.29s  || +0m00.13s | +0.75%
0m15.12s  | Experiments/NewPipeline/ExtractionOCaml/word_by_word_montgomery      | 0m14.96s  || +0m00.15s | +1.06%
0m14.43s  | secp256k1_32.c                                                       | 0m14.22s  || +0m00.20s | +1.47%
0m14.19s  | p256_32.c                                                            | 0m14.46s  || -0m00.27s | -1.86%
0m12.72s  | Experiments/NewPipeline/CStringification.vo                          | 0m12.80s  || -0m00.08s | -0.62%
0m10.88s  | p384_64.c                                                            | 0m10.99s  || -0m00.10s | -1.00%
0m09.16s  | Experiments/NewPipeline/ExtractionOCaml/unsaturated_solinas          | 0m08.87s  || +0m00.29s | +3.26%
0m09.14s  | Experiments/NewPipeline/ExtractionOCaml/word_by_word_montgomery.ml   | 0m09.33s  || -0m00.18s | -2.03%
0m07.96s  | Experiments/NewPipeline/GENERATEDIdentifiersWithoutTypes.vo          | 0m07.96s  || +0m00.00s | +0.00%
0m06.61s  | p224_32.c                                                            | 0m06.52s  || +0m00.09s | +1.38%
0m06.37s  | Experiments/NewPipeline/ExtractionOCaml/unsaturated_solinas.ml       | 0m06.29s  || +0m00.08s | +1.27%
0m05.96s  | Experiments/NewPipeline/ExtractionOCaml/saturated_solinas            | 0m05.60s  || +0m00.36s | +6.42%
0m05.92s  | Experiments/NewPipeline/ExtractionHaskell/word_by_word_montgomery.hs | 0m05.82s  || +0m00.09s | +1.71%
0m04.70s  | Experiments/NewPipeline/ExtractionHaskell/unsaturated_solinas.hs     | 0m04.35s  || +0m00.35s | +8.04%
0m04.50s  | Experiments/NewPipeline/ExtractionOCaml/saturated_solinas.ml         | 0m04.63s  || -0m00.12s | -2.80%
0m03.82s  | Experiments/NewPipeline/ExtractionHaskell/saturated_solinas.hs       | 0m03.62s  || +0m00.19s | +5.52%
0m02.62s  | Experiments/NewPipeline/MiscCompilerPassesProofs.vo                  | 0m02.56s  || +0m00.06s | +2.34%
0m02.31s  | curve25519_32.c                                                      | 0m02.40s  || -0m00.08s | -3.74%
0m02.09s  | secp256k1_64.c                                                       | 0m02.18s  || -0m00.09s | -4.12%
0m02.05s  | p224_64.c                                                            | 0m02.04s  || +0m00.00s | +0.49%
0m01.96s  | p256_64.c                                                            | 0m01.94s  || +0m00.02s | +1.03%
0m01.56s  | curve25519_64.c                                                      | 0m01.54s  || +0m00.02s | +1.29%
0m01.53s  | Experiments/NewPipeline/CLI.vo                                       | 0m01.57s  || -0m00.04s | -2.54%
0m01.26s  | Experiments/NewPipeline/StandaloneHaskellMain.vo                     | 0m01.26s  || +0m00.00s | +0.00%
0m01.22s  | Experiments/NewPipeline/Language.vo                                  | 0m01.26s  || -0m00.04s | -3.17%
0m01.22s  | Experiments/NewPipeline/StandaloneOCamlMain.vo                       | 0m01.21s  || +0m00.01s | +0.82%
0m01.08s  | Experiments/NewPipeline/CompilersTestCases.vo                        | 0m00.99s  || +0m00.09s | +9.09%
0m01.06s  | Experiments/NewPipeline/AbstractInterpretation.vo                    | 0m01.02s  || +0m00.04s | +3.92%
0m00.87s  | Experiments/NewPipeline/RewriterProofs.vo                            | 0m00.97s  || -0m00.09s | -10.30%
0m00.74s  | Experiments/NewPipeline/MiscCompilerPasses.vo                        | 0m00.72s  || +0m00.02s | +2.77%
0m00.48s  | Experiments/NewPipeline/UnderLets.vo                                 | 0m00.52s  || -0m00.04s | -7.69%

src/Experiments/NewPipeline/UnderLetsProofs.v
@@ -333,6 +333,18 @@ Module Compilers.
                                  @interp _ (f xv)
              end.
 
+        Fixpoint interp_related {T1 T2} (R : T1 -> T2 -> Prop) (e : UnderLets T1) (v2 : T2) : Prop
+          := match e with
+             | Base v1 => R v1 v2
+             | UnderLet t e f (* combine the App rule with the Abs rule *)
+               => exists fv ev,
+                  expr.interp_related ident_interp e ev
+                  /\ (forall x1 x2,
+                         x1 == x2
+                         -> @interp_related T1 T2 R (f x1) (fv x2))
+                  /\ fv ev = v2
+             end.
+
         Lemma interp_splice {A B} (x : UnderLets A) (e : A -> UnderLets B)
           : interp (splice x e) = interp (e (interp x)).
         Proof. induction x; cbn [splice interp]; eauto. Qed.
@@ -352,6 +364,201 @@ Module Compilers.
         Lemma interp_of_expr {t} (x : expr t)
           : expr.interp ident_interp (interp (of_expr x)) = expr.interp ident_interp x.
         Proof. induction x; cbn [expr.interp interp of_expr]; cbv [LetIn.Let_In]; eauto. Qed.
+
+        Lemma to_expr_interp_related_iff {t e v}
+          : interp_related (expr.interp_related ident_interp (t:=t)) e v
+            <-> expr.interp_related ident_interp (UnderLets.to_expr e) v.
+        Proof using Type.
+          revert v; induction e; cbn [UnderLets.to_expr interp_related expr.interp_related]; try reflexivity.
+          setoid_rewrite H.
+          reflexivity.
+        Qed.
+
+        Global Instance interp_related_Proper_iff {T1 T2}
+          : Proper (pointwise_relation _ (pointwise_relation _ iff) ==> eq ==> eq ==> iff) (@interp_related T1 T2) | 10.
+        Proof using Type.
+          cbv [pointwise_relation respectful Proper].
+          intros R1 R2 HR x y ? x' y' H'; subst y y'.
+          revert x'; induction x; [ apply HR | ]; cbn [interp_related].
+          setoid_rewrite H; reflexivity.
+        Qed.
+
+        Lemma splice_interp_related_iff {A B T R x e} {v : T}
+          : interp_related R (@UnderLets.splice _ ident _ A B x e) v
+            <-> interp_related
+                  (fun xv => interp_related R (e xv))
+                  x v.
+        Proof using Type.
+          revert v; induction x; cbn [UnderLets.splice interp_related]; [ reflexivity | ].
+          match goal with H : _ |- _ => setoid_rewrite H end.
+          reflexivity.
+        Qed.
+
+        Lemma splice_list_interp_related_iff_gen {A B T R x e1 e2 base} {v : T}
+              (He1e2 : forall ls', e1 ls' = e2 (base ++ ls'))
+          : interp_related R (@UnderLets.splice_list _ ident _ A B x e1) v
+            <-> list_rect
+                  (fun _ => list _ -> _ -> Prop)
+                  (fun ls v => interp_related R (e2 ls) v)
+                  (fun x xs recP ls v
+                   => interp_related
+                        (fun x' v => recP (ls ++ [x']) v)
+                        x
+                        v)
+                  x
+                  base
+                  v.
+        Proof using Type.
+          revert base v e1 e2 He1e2; induction x as [|? ? IHx]; cbn [UnderLets.splice_list interp_related list_rect]; intros.
+          { intros; rewrite He1e2, ?app_nil_r; reflexivity. }
+          { setoid_rewrite splice_interp_related_iff.
+            apply interp_related_Proper_iff; [ | reflexivity.. ]; cbv [pointwise_relation]; intros.
+            specialize (fun v => IHx (base ++ [v])).
+            setoid_rewrite IHx; [ reflexivity | ].
+            intros; rewrite He1e2, <- ?app_assoc; reflexivity. }
+        Qed.
+
+        Lemma splice_list_interp_related_iff {A B T R x e} {v : T}
+          : interp_related R (@UnderLets.splice_list _ ident _ A B x e) v
+            <-> list_rect
+                  (fun _ => list _ -> _ -> Prop)
+                  (fun ls v => interp_related R (e ls) v)
+                  (fun x xs recP ls v
+                   => interp_related
+                        (fun x' v => recP (ls ++ [x']) v)
+                        x
+                        v)
+                  x
+                  nil
+                  v.
+        Proof using Type.
+          apply splice_list_interp_related_iff_gen; reflexivity.
+        Qed.
+
+        Lemma splice_interp_related_of_ex {A B T T' RA RB x e} {v : T}
+          : (exists ev (xv : T'),
+                interp_related RA x xv
+                /\ (forall x1 x2,
+                       RA x1 x2
+                       -> interp_related RB (e x1) (ev x2))
+                /\ ev xv = v)
+            -> interp_related RB (@UnderLets.splice _ ident _ A B x e) v.
+        Proof using Type.
+          revert e v; induction x; cbn [interp_related UnderLets.splice]; intros.
+          all: repeat first [ progress destruct_head'_ex
+                            | progress destruct_head'_and
+                            | progress subst
+                            | reflexivity
+                            | match goal with
+                              | [ H : _ |- _ ] => apply H; clear H
+                              end ].
+          do 2 eexists; repeat apply conj; [ eassumption | | ]; intros.
+          { match goal with H : _ |- _ => apply H; clear H end.
+            do 2 eexists; repeat apply conj; now eauto. }
+          { reflexivity. }
+        Qed.
+
+        Lemma splice_list_interp_related_of_ex {A B T T' RA RB x e} {v : T}
+          : (exists ev (xv : list T'),
+                    List.Forall2 (interp_related RA) x xv
+                    /\ (forall x1 x2,
+                           List.length x2 = List.length xv
+                           -> List.Forall2 RA x1 x2
+                           -> interp_related RB (e x1) (ev x2))
+                    /\ ev xv = v)
+            -> interp_related RB (@UnderLets.splice_list _ ident _ A B x e) v.
+        Proof using Type.
+          revert e v; induction x as [|x xs IHxs]; cbn [interp_related UnderLets.splice_list]; intros.
+          all: repeat first [ progress destruct_head'_ex
+                            | progress destruct_head'_and
+                            | progress cbn [List.length] in *
+                            | progress subst
+                            | reflexivity
+                            | match goal with
+                              | [ H : List.Forall2 _ nil ?x |- _ ] => is_var x; inversion H; clear H
+                              | [ H : List.Forall2 _ (cons _ _) ?x |- _ ] => is_var x; inversion H; clear H
+                              | [ |- List.Forall2 _ _ _ ] => constructor
+                              | [ H : _ |- _ ] => apply H; clear H
+                              end ].
+          lazymatch goal with
+          | [ H : forall l1 l2, length l2 = S (length _) -> Forall2 _ l1 l2 -> _ |- _ ]
+            => specialize (fun l ls l' ls' (pf0 : length _ = _) pf1 pf2 => H (cons l ls) (cons l' ls') (f_equal S pf0) (Forall2_cons _ _ pf1 pf2))
+          end.
+          eapply splice_interp_related_of_ex; do 2 eexists; repeat apply conj;
+            intros; [ eassumption | | ].
+          { eapply IHxs.
+            do 2 eexists; repeat apply conj; intros;
+              [ eassumption | | ].
+            { match goal with H : _ |- _ => eapply H; clear H end; eassumption. }
+            { reflexivity. } }
+          { reflexivity. }
+        Qed.
+
+        Lemma list_rect_interp_related {A B Pnil Pcons ls B' Pnil' Pcons' ls' R}
+              (Hnil : interp_related R Pnil Pnil')
+              (Hcons : forall x x',
+                  expr.interp_related ident_interp x x'
+                  -> forall l l',
+                    List.Forall2 (expr.interp_related ident_interp) l l'
+                    -> forall rec rec',
+                      interp_related R rec rec'
+                      -> interp_related R (Pcons x l rec) (Pcons' x' l' rec'))
+              (Hls : List.Forall2 (expr.interp_related ident_interp (t:=A)) ls ls')
+          : interp_related
+              R
+              (list_rect
+                 (fun _ : list _ => UnderLets B)
+                 Pnil
+                 Pcons
+                 ls)
+              (list_rect
+                 (fun _ : list _ => B')
+                 Pnil'
+                 Pcons'
+                 ls').
+        Proof using Type. induction Hls; cbn [list_rect] in *; auto. Qed.
+
+        Lemma nat_rect_interp_related {A PO PS n A' PO' PS' n' R}
+              (Hnil : interp_related R PO PO')
+              (Hcons : forall n rec rec',
+                  interp_related R rec rec'
+                  -> interp_related R (PS n rec) (PS' n rec'))
+              (Hn : n = n')
+          : interp_related
+              R
+              (nat_rect (fun _ => UnderLets A) PO PS n)
+              (nat_rect (fun _ => A') PO' PS' n').
+        Proof using Type. subst n'; induction n; cbn [nat_rect] in *; auto. Qed.
+
+        Lemma nat_rect_arrow_interp_related {A B PO PS n x A' B' PO' PS' n' x' R}
+              {R' : A -> A' -> Prop}
+              (Hnil : forall x x', R' x x' -> interp_related R (PO x) (PO' x'))
+              (Hcons : forall n rec rec',
+                  (forall x x', R' x x' -> interp_related R (rec x) (rec' x'))
+                  -> forall x x',
+                    R' x x'
+                    -> interp_related R (PS n rec x) (PS' n rec' x'))
+              (Hn : n = n')
+              (Hx : R' x x')
+          : interp_related
+              R
+              (nat_rect (fun _ => A -> UnderLets B) PO PS n x)
+              (nat_rect (fun _ => A' -> B') PO' PS' n' x').
+        Proof using Type. subst n'; revert x x' Hx; induction n; cbn [nat_rect] in *; auto. Qed.
+
+        Lemma interp_related_Proper_impl_same_UnderLets {A B B' R1 R2 e v f}
+              (HR : forall e v, (R1 e v : Prop) -> (R2 e (f v) : Prop))
+          : @interp_related A B R1 e v
+            -> @interp_related A B' R2 e (f v).
+        Proof using Type.
+          revert f v HR; induction e; cbn [interp_related]; [ now eauto | ]; intros F v HR H'.
+          destruct H' as [fv H']; exists (fun ev => F (fv ev)).
+          repeat first [ let x := fresh "x" in destruct H' as [x H']; exists x
+                       | let x := fresh "x" in intro x; specialize (H' x)
+                       | let H := fresh "H" in destruct H' as [H H']; split; [ exact H || now subst | ]
+                       | let H := fresh "H" in destruct H' as [H' H]; split; [ | exact H || now subst ] ].
+          auto.
+        Qed.
       End for_interp.
 
       Section for_interp2.
